\large
\begin{equation}
y[n]= \sum _{m=0} ^L b[m] \cdot x[n-m]+ \sum _ {r=1} ^R a[r] \cdot y(n-r)
\end{equation}

\large
H(z)=\dfrac{Y(z)}  {X(z)}= \dfrac{\sum _ {m=0} ^L b(m)  \cdot z^{-m}}{1-\sum _ {r=1} ^ R a(r) \cdot z^{-r}}

\large
\begin{equation}
y[n]= x[n] + \sum _{r=1}^2 a[r] \cdot y[n-r]
\end{equation}

\large
H(z)=\dfrac{1}  {1-a_1\cdot z^{-1}-a_2\cdot z^{-2}}

\large
\Omega=\dfrac{2\pi\cdot 440 Hz}{8000 Hz}

\large
p_{0,1}=Q \cdot \exp\left(\pm j \cdot Q\right)

\large
H(z)=\dfrac{1}  {1-a_1\cdot z^{-1}-a_2\cdot z^{-2}} =\dfrac{1}  {(1-p_0\cdot z^{-1})(1-p_1\cdot z^{-1})}

\large
a_1=(p_0+p_1) \\
\large
a_2=p_0\cdot p_1

\large
a_1=2Q\cdot \cos(\Omega)\\
\large
a_2=-Q^2

\large
h_t=tanh(W_{ih}\cdot  x_t+b_{ih}+W_{hh}\cdot h_{t−1}+b_{hh})

\large
h_t[i]=y[t−i] \text{ for i=0,1,2}

\large
h_t[0]=y[t]=x[t]+a_1 \cdot y[t−1] + a_2 \cdot y[t−2]

\large
h_t[0]=x[t]+a_1 \cdot h_{t−1} [0]+a_2 \cdot h_{t−1} [1]

\large
h_t[1]=h_{t−1}[0] \\
\large
h_t [2]=h_{t−1}[1]

\large
h_t=W_{ih} \cdot x_t+W_{hh} \cdot h_{t−1}

\large
W_{hh}=
\begin{bmatrix}
a_1 & a_2 & 0\\
1 & 0 & 0 \\
0 & 1 & 0
\end{bmatrix}

\large
W_{ih}=
\begin{bmatrix}
 1\\
0 \\
0
\end{bmatrix}